WinningRegion and comments

PositionalDeterminacy/Attractor.thy
@@ -10,31 +10,27 @@ text {* Here we define the @{term p}-attractor of a set of vertices. *}
 
 context ParityGame begin
 
+text {* We define the conditions for a vertex to be directly attracted from a given set. *}
 definition directly_attracted :: "Player \<Rightarrow> 'a set \<Rightarrow> 'a set" where
-  "directly_attracted p W \<equiv> {v \<in> V - W. \<not>deadend v \<and>
-      (v \<in> VV p   \<longrightarrow> (\<exists>w. v\<rightarrow>w \<and> w \<in> W))
-    \<and> (v \<in> VV p** \<longrightarrow> (\<forall>w. v\<rightarrow>w \<longrightarrow> w \<in> W))}"
+  "directly_attracted p S \<equiv> {v \<in> V - S. \<not>deadend v \<and>
+      (v \<in> VV p   \<longrightarrow> (\<exists>w. v\<rightarrow>w \<and> w \<in> S))
+    \<and> (v \<in> VV p** \<longrightarrow> (\<forall>w. v\<rightarrow>w \<longrightarrow> w \<in> S))}"
 
 abbreviation "attractor_step p W S \<equiv> W \<union> S \<union> directly_attracted p S"
 
-text {* The attractor set of a given set of vertices, defined as a least fixed point. *}
+text {* The @{text p}-attractor set of @{text W}, defined as a least fixed point. *}
 definition attractor :: "Player \<Rightarrow> 'a set \<Rightarrow> 'a set" where
   "attractor p W = lfp (attractor_step p W)"
 
+subsection {* @{const directly_attracted} *}
+
+text {* Show a few basic properties of @{const directly_attracted}. *}
 lemma directly_attracted_disjoint     [simp]: "directly_attracted p W \<inter> W = {}"
   and directly_attracted_empty        [simp]: "directly_attracted p {} = {}"
   and directly_attracted_V_empty      [simp]: "directly_attracted p V = {}"
   and directly_attracted_bounded_by_V [simp]: "directly_attracted p W \<subseteq> V"
   and directly_attracted_contains_no_deadends [elim]: "v \<in> directly_attracted p W \<Longrightarrow> \<not>deadend v"
-  using directly_attracted_def by auto
-
-lemma directly_attracted_union:
-  assumes "v \<in> directly_attracted p W" "v \<notin> U"
-  shows "v \<in> directly_attracted p (W \<union> U)"
-proof-
-  have "v \<in> V - (W \<union> U)" using assms unfolding directly_attracted_def by auto
-  thus ?thesis using assms(1) unfolding directly_attracted_def by auto
-qed
+  unfolding directly_attracted_def by blast+
 
 subsection {* @{text attractor_step} *}
 
@@ -42,8 +38,10 @@ lemma attractor_step_empty: "attractor_step p {} {} = {}"
   and attractor_step_bounded_by_V: "\<lbrakk> W \<subseteq> V; S \<subseteq> V \<rbrakk> \<Longrightarrow> attractor_step p W S \<subseteq> V"
   by simp_all
 
-lemma mono_restriction_is_mono: "mono f \<Longrightarrow> mono (\<lambda>S. f (S \<inter> V))"
-  unfolding mono_def by (meson inf_mono monoD subset_refl)
+text {*
+  The definition of @{const attractor} uses @{const lfp}.  For this to be well-defined, we
+  need show that @{text attractor_step} is monotone.
+*}
 
 lemma attractor_step_mono: "mono (attractor_step p W)"
 proof (rule monoI)
@@ -58,67 +56,19 @@ proof (rule monoI)
   qed
 qed
 
-subsection {* @{term attractor} *}
+subsection {* Basic properties of @{term attractor} *}
 
 lemma attractor_unfolding: "attractor p W = attractor_step p W (attractor p W)"
   unfolding attractor_def using attractor_step_mono lfp_unfold by blast
 lemma attractor_lowerbound: "attractor_step p W S \<subseteq> S \<Longrightarrow> attractor p W \<subseteq> S"
   unfolding attractor_def using attractor_step_mono by (simp add: lfp_lowerbound)
-
-text {* A powerful induction schema for @{term attractor}. *}
-lemma attractor_set_induction [consumes 1, case_names step union]:
-  assumes "W \<subseteq> V"
-    and step: "\<And>S. S \<subseteq> V \<Longrightarrow> P S \<Longrightarrow> P (attractor_step p W S)"
-    and union: "\<And>M. \<forall>S \<in> M. S \<subseteq> V \<and> P S \<Longrightarrow> P (\<Union>M)"
-  shows "P (attractor p W)"
-proof-
-  let ?P = "\<lambda>S. P (S \<inter> V)"
-  let ?f = "\<lambda>S. attractor_step p W (S \<inter> V)"
-  let ?A = "lfp ?f"
-  let ?B = "lfp (attractor_step p W)"
-  have f_mono: "mono ?f"
-    using mono_restriction_is_mono[of "attractor_step p W"] attractor_step_mono by simp
-  have P_A: "?P ?A" proof (rule lfp_ordinal_induct_set)
-    show "\<And>S. ?P S \<Longrightarrow> ?P (W \<union> (S \<inter> V) \<union> directly_attracted p (S \<inter> V))"
-      by (metis assms(1) attractor_step_bounded_by_V inf.absorb1 inf_le2 local.step)
-    show "\<And>M. \<forall>S \<in> M. ?P S \<Longrightarrow> ?P (\<Union>M)" proof-
-      fix M
-      let ?M = "{S \<inter> V | S. S \<in> M}"
-      assume "\<forall>S\<in>M. ?P S"
-      hence "\<forall>S \<in> ?M. S \<subseteq> V \<and> P S" by auto
-      hence *: "P (\<Union>?M)" by (simp add: union)
-      have "\<Union>?M = (\<Union>M) \<inter> V" by blast
-      thus "?P (\<Union>M)" using * by auto
-    qed
-  qed (insert f_mono)
-
-  have *: "W \<union> (V \<inter> V) \<union> directly_attracted p (V \<inter> V) \<subseteq> V"
-    using `W \<subseteq> V` attractor_step_bounded_by_V by auto
-  have "?A \<subseteq> V" "?B \<subseteq> V" using * by (simp_all add: lfp_lowerbound)
-
-  have "?A = ?f ?A" using f_mono lfp_unfold by blast
-  hence "?A = W \<union> (?A \<inter> V) \<union> directly_attracted p (?A \<inter> V)" using `?A \<subseteq> V` by simp
-  hence *: "attractor_step p W ?A \<subseteq> ?A" using `?A \<subseteq> V` inf.absorb1 by fastforce
-
-  have "?B = attractor_step p W ?B" using attractor_step_mono lfp_unfold by blast
-  hence "?f ?B \<subseteq> ?B" using `?B \<subseteq> V` by (metis (no_types, lifting) equalityD2 le_iff_inf)
-
-  have "?A = ?B" proof
-    show "?A \<subseteq> ?B" using `?f ?B \<subseteq> ?B` by (simp add: lfp_lowerbound)
-    show "?B \<subseteq> ?A" using * by (simp add: lfp_lowerbound)
-  qed
-  hence "?P ?B" using P_A by (simp add: attractor_def)
-  thus ?thesis using `?B \<subseteq> V` by (simp add: attractor_def le_iff_inf)
-qed
-
 lemma attractor_set_non_empty: "W \<noteq> {} \<Longrightarrow> attractor p W \<noteq> {}"
   and attractor_set_base: "W \<subseteq> attractor p W"
   using attractor_unfolding by auto
-
 lemma attractor_in_V: "W \<subseteq> V \<Longrightarrow> attractor p W \<subseteq> V"
   using attractor_lowerbound attractor_step_bounded_by_V by auto
 
-subsection {* Extension theorems *}
+subsection {* Attractor set extensions *}
 
 lemma attractor_set_VVp:
   assumes "v \<in> VV p" "v\<rightarrow>w" "w \<in> attractor p W"
@@ -192,6 +142,64 @@ next
     }
     thus False using v by blast
   qed
+qed
+
+subsection {* Attractor set induction *}
+
+lemma mono_restriction_is_mono: "mono f \<Longrightarrow> mono (\<lambda>S. f (S \<inter> V))"
+  unfolding mono_def by (meson inf_mono monoD subset_refl)
+
+text {*
+  We prove a powerful induction schema for @{term attractor}.  Being able to prove this is the
+  only reason why we do not use @{text inductive_set} to define the attractor set, because I was
+  unable to prove this schema with @{text inductive_set} alone (without @{const lfp}).
+
+  If you know how to get this induction schema working with @{text inductive_set} and without
+  @{const lfp} (and thus hopefully with a shorter proof), please contact the maintainer.
+*}
+lemma attractor_set_induction [consumes 1, case_names step union]:
+  assumes "W \<subseteq> V"
+    and step: "\<And>S. S \<subseteq> V \<Longrightarrow> P S \<Longrightarrow> P (attractor_step p W S)"
+    and union: "\<And>M. \<forall>S \<in> M. S \<subseteq> V \<and> P S \<Longrightarrow> P (\<Union>M)"
+  shows "P (attractor p W)"
+proof-
+  let ?P = "\<lambda>S. P (S \<inter> V)"
+  let ?f = "\<lambda>S. attractor_step p W (S \<inter> V)"
+  let ?A = "lfp ?f"
+  let ?B = "lfp (attractor_step p W)"
+  have f_mono: "mono ?f"
+    using mono_restriction_is_mono[of "attractor_step p W"] attractor_step_mono by simp
+  have P_A: "?P ?A" proof (rule lfp_ordinal_induct_set)
+    show "\<And>S. ?P S \<Longrightarrow> ?P (W \<union> (S \<inter> V) \<union> directly_attracted p (S \<inter> V))"
+      by (metis assms(1) attractor_step_bounded_by_V inf.absorb1 inf_le2 local.step)
+    show "\<And>M. \<forall>S \<in> M. ?P S \<Longrightarrow> ?P (\<Union>M)" proof-
+      fix M
+      let ?M = "{S \<inter> V | S. S \<in> M}"
+      assume "\<forall>S\<in>M. ?P S"
+      hence "\<forall>S \<in> ?M. S \<subseteq> V \<and> P S" by auto
+      hence *: "P (\<Union>?M)" by (simp add: union)
+      have "\<Union>?M = (\<Union>M) \<inter> V" by blast
+      thus "?P (\<Union>M)" using * by auto
+    qed
+  qed (insert f_mono)
+
+  have *: "W \<union> (V \<inter> V) \<union> directly_attracted p (V \<inter> V) \<subseteq> V"
+    using `W \<subseteq> V` attractor_step_bounded_by_V by auto
+  have "?A \<subseteq> V" "?B \<subseteq> V" using * by (simp_all add: lfp_lowerbound)
+
+  have "?A = ?f ?A" using f_mono lfp_unfold by blast
+  hence "?A = W \<union> (?A \<inter> V) \<union> directly_attracted p (?A \<inter> V)" using `?A \<subseteq> V` by simp
+  hence *: "attractor_step p W ?A \<subseteq> ?A" using `?A \<subseteq> V` inf.absorb1 by fastforce
+
+  have "?B = attractor_step p W ?B" using attractor_step_mono lfp_unfold by blast
+  hence "?f ?B \<subseteq> ?B" using `?B \<subseteq> V` by (metis (no_types, lifting) equalityD2 le_iff_inf)
+
+  have "?A = ?B" proof
+    show "?A \<subseteq> ?B" using `?f ?B \<subseteq> ?B` by (simp add: lfp_lowerbound)
+    show "?B \<subseteq> ?A" using * by (simp add: lfp_lowerbound)
+  qed
+  hence "?P ?B" using P_A by (simp add: attractor_def)
+  thus ?thesis using `?B \<subseteq> V` by (simp add: attractor_def le_iff_inf)
 qed
 
 end -- "context ParityGame"
